\section{Problem 1 (3 points)}
Two signals $x[n]$ and $y[n]$ are given by


\begin{equation*}
    x[n]=\left\{\begin{array}{ll}2 & n=0 \\ 1 & n= \pm 1 \\ 0 & \text { otherwise, }\end{array} \quad y[n]=\left\{\begin{array}{ll}1 & -M \leq n \leq M \\ 0 & \text { otherwise }\end{array}\right.\right. 
\end{equation*}

\subsection*{(a) Show that the Fourier transform of $x[n]$ is given by... and sketch it for $\omega \in [-\pi , \pi]$.}

\begin{equation*}
    X(\omega)=2+2 \cos{\omega}
\end{equation*}

We have that

\begin{equation*}
    X(\omega)=\sum_{n=-\infty}^\infty x[n]e^{-j\omega n}
\end{equation*}

In our case we can write

\begin{equation*}
    X(\omega)=\sum_{n=-1}^1 x[n]e^{-j\omega n} = -e^{j\omega}+ 2 + e^{-j\omega}
\end{equation*}

From Euler's formula we get that

\begin{equation*}
    \cos{x} = \frac{e^{ix}+e^{-ix}}{2}
\end{equation*}

by combining these two we get:

\begin{equation*}
    X(\omega)=2+2 \cos{\omega}
\end{equation*}

\importimage{1a}

\subsection*{(b) Show that the Fourier transform of y[n] is given by}

\begin{equation*}
    Y(\omega)=\frac{\sin \left(\omega\left(M+\frac{1}{2}\right)\right)}{\sin \left(\frac{\omega}{2}\right)} 
\end{equation*}

\textbf{and sketch it for $M=10$ and $\omega \in [-\pi,\pi]$}

\begin{equation*}
    Y(\omega)=\sum_{n=-M}^M e^{-j\omega n}
\end{equation*}

This is a finite geometric series. By using the general formula for a geometric series
\begin{equation*}
    \sum_{k=m}^{n} a r^{k}=\left\{\begin{array}{ll}a(n-m+1) & \text { if } r=1 \\ \frac{a\left(r^{m}-r^{n+1}\right)}{1-r} & \text { if } r \neq 1\end{array}\right. 
\end{equation*}

we get
\begin{equation*}
    Y(\omega)=\frac{e^{j\omega M}-e^{-j\omega (M+1)}}{1-e^{-j\omega}}
\end{equation*}